abstaction context terms

src/EvalExecs/TransferFrom.v
@@ -4,8 +4,8 @@ Require Import UMLang.ExecGenerator.
 
 Require Import EIP20.
 Require Import Common.
+Require Import Templates.TransferFrom.
 Import EIP20.
-
 
 Definition transferFrom_ls_template_exec_sig (_from :  address)
                                              (_to :  address)
@@ -23,51 +23,64 @@ Definition transferFrom_ls_template_exec (_from :  address)
   let_term_of_2_fast @transferFrom_ls_template_exec_sig (transferFrom_ls_template_exec_sig _from _to _value l).
 Defined.
 
-(* Definition transferFrom_ls_template_exec (_from :  address)
-                                         (_to :  address)
-                                         (_value :  uint256)
-                                         (l : LedgerLRecord rec) : LedgerLRecord rec.
-  flat_term_of_2 @transferFromTemplate_exec_let (transferFromTemplate_exec_let _from _to _value l).
-Defined. *)
-
-Definition transferFrom_ls_template_exec_prf (_from :  address)
-                                             (_to :  address) 
-                                             (_value :  uint256) 
-                                             (l : LedgerLRecord rec) :
+Lemma transferFrom_ls_template_exec_prf : forall (_from :  address)
+                                                 (_to :  address) 
+                                                 (_value :  uint256) 
+                                                 (l : LedgerLRecord rec),
   transferFrom_ls_template_exec _from _to _value l = 
   exec_state (Uinterpreter (@transferFrom_ls_template rec def _ _ _ _ _from _to _value)) l.
+Proof.
+  intros.  
   proof_of_2 transferFrom_ls_template_exec transferFrom_ls_template_exec_sig 
              (transferFrom_ls_template_exec_sig _from _to _value l).
+Qed.
+
+Definition transferFrom_ls_pre_payload_computed' 
+                              (_from :  address)
+                              (_to :  address) 
+                              (_value :  uint256)
+                              (l: LedgerLRecord rec): True.
+    assert (LedgerLRecord rec).
+    remember (transferFrom_ls_template_exec _from _to _value {$$ l with Ledger_LocalState := default $$}) as exec.
+    destruct_ledger l.
+
+    time "transferFrom_ls_template_exec unfold" unfold transferFrom_ls_template_exec in Heqexec. idtac.
+    
+    time "remember" match goal with
+    | Heql0 : exec = ?L |- _ => match L with
+                                | context [exec_state (Uinterpreter (transferFrom_ls_payload rec def _ _ _ _ _ )) ?LL] => 
+                                        remember LL as pre_exec
+                                end
+    end. idtac.
+
+    time "transferFrom_ls_pre_payload_computed compute" vm_compute in Heqpre_exec. idtac.
+    match goal with
+    | Heql0: pre_exec = ?LL |- _ => transparent_abstract exact_no_check LL using transferFrom_ls_pre_payload_computed_curried
+    end.
+    exact I.
 Defined.
 
 
-Definition transferFrom_ls_pre_payload_computed: 
-                       forall (_from :  address)
+Definition transferFrom_ls_pre_payload_computed
+                              (_from :  address)
                               (_to :  address) 
                               (_value :  uint256)
-                              (l: LedgerLRecord rec), LedgerLRecord rec.
-    (* {t: LedgerLRecord rec | t = transferFromTemplate_exec _from _to _value {$$ l with Ledger_LocalState := default $$}}. *)
-Proof.
-    intros.
-    remember (transferFrom_ls_template_exec _from _to _value {$$ l with Ledger_LocalState := default $$}).
-
-    destruct l. repeat destruct p.
-    destruct v. repeat destruct p.
-    destruct c. repeat destruct p. idtac.
-
-    time "transferFrom_ls_template_exec unfold" unfold transferFrom_ls_template_exec in Heql0. idtac.
-    
-    time "remember" match goal with
-    | Heql0 : l0 = ?L |- _ => match L with
-                              | context [exec_state (Uinterpreter (transferFrom_ls_payload rec def _ _ _ _ _ )) ?LL] => 
-                                        remember LL
-                              end
-    end. idtac.
-
-    time "transferFrom_ls_pre_payload_computed compute" vm_compute in Heql3. idtac.
-    match goal with
-    | Heql0: l3 = ?LL |- _ => exact LL
-    end.
+                              (l: LedgerLRecord rec): LedgerLRecord rec.     
+remember l as ledger. destruct_ledger l.
+refine (uncurry (f:=_GlobalClass) (transferFrom_ls_pre_payload_computed_curried _from _to _value)
+      (s, (s0, (s1, (s2, (s3, (s4,
+             (c0,
+              (m,
+               (m0,
+                (v0,
+                 (v1,
+                  (v2,
+                   (v3,
+                    (v4,
+                     (v5,
+                      (v6,
+                       (v7, (v8, (v9, (v10, (v11, (v12, (v13, (v14, (v15, (v16, (v17,
+                       l1)))))))))))))))))))))))))))%xprod).
 Defined.
 
 Lemma transferFrom_ls_template_by_payload: 
@@ -80,171 +93,67 @@ Lemma transferFrom_ls_template_by_payload:
   let _value := local_left_field _ _ _ ("_value", 1%nat) in
   let _allowance := local_left_field _ _ _ ("allowance", 1%nat) in
   let _success := local_left_field _ _ _ ("success", 1%nat) in
-  let l0 := transferFrom_ls_pre_payload_computed _from_value _to_value _value_value l in  
+  let pre_exec := transferFrom_ls_pre_payload_computed _from_value _to_value _value_value l in  
 
   transferFrom_ls_template_exec _from_value _to_value _value_value {$$ l with Ledger_LocalState := default $$} =
-  exec_state (Uinterpreter (@transferFrom_ls_payload rec def _  _from _to _value _success _allowance)) l0.
+  exec_state (Uinterpreter (@transferFrom_ls_payload rec def _  _from _to _value _success _allowance)) pre_exec.
 Proof.
   intros.
-  (* remember (transferFrom_ls_template_exec _from _to _value {$$ l with Ledger_LocalState := default $$}). *)
-
-  destruct l. repeat destruct p.
-  destruct v. repeat destruct p.
-  destruct c. repeat destruct p. idtac.
-
-  time "transferFrom_ls_template_exec unfold" unfold transferFrom_ls_template_exec. idtac.
-    
+  destruct_ledger l.
+  time "transferFrom_ls_template_exec unfold" unfold transferFrom_ls_template_exec. idtac.  
   time "remember" match goal with
     | |- context [exec_state (Uinterpreter (transferFrom_ls_payload rec def ?a1 ?a2 ?a3 ?a4 ?a5 )) ?LL] => 
-                                        remember LL  
+                                        remember LL as pre_exec' 
   end. idtac.
 
-  time "transferFrom_ls_pre_payload_computed compute" vm_compute in Heql3. idtac.
+  time "transferFrom_ls_pre_payload_computed compute" vm_compute in Heqpre_exec'. idtac.
 
   time "remember" match goal with
   | |- context [exec_state (Uinterpreter (transferFrom_ls_payload rec def ?a1 ?a2 ?a3 ?a4 ?a5 )) ?LL] => 
-                                      remember a1                            
+                                      remember a1 as u1
   end. idtac.
 
   time "remember" match goal with
   | |- context [exec_state (Uinterpreter (transferFrom_ls_payload rec def ?a1 ?a2 ?a3 ?a4 ?a5 )) ?LL] => 
-                                        remember a2
+                                        remember a2 as u2
   
   end. idtac.
 
   time "remember" match goal with
   | |- context [exec_state (Uinterpreter (transferFrom_ls_payload rec def ?a1 ?a2 ?a3 ?a4 ?a5 )) ?LL] => 
-                                      remember a3                        
+                                      remember a3 as u3
   end. idtac.
 
   time "remember" match goal with
   | |- context [exec_state (Uinterpreter (transferFrom_ls_payload rec def ?a1 ?a2 ?a3 ?a4 ?a5 )) ?LL] => 
-                                      remember a4
+                                      remember a4 as u4
   end. idtac.
 
   time "remember" match goal with
   | |- context [exec_state (Uinterpreter (transferFrom_ls_payload rec def ?a1 ?a2 ?a3 ?a4 ?a5 )) ?LL] => 
-                                      remember a5
+                                      remember a5 as u5
   end. idtac.
 
-  assert (forall l, exec_state (sRReader (ULtoRValue u2)) l = l). 
-  intros. 
-  subst u2. auto.
-
+  assert (forall l, exec_state (sRReader (ULtoRValue u4)) l = l). 
+  intros. subst u4. auto.
   rewrite H.
 
-  assert (forall X (x:X) (b: bool), 
-    (if b then x else x) = x). intros; destruct b; auto.
+  assert (forall X (x:X) (b: bool), (if b then x else x) = x). intros; destruct b; auto.
   rewrite H0.
 
-  assert (u = _from) by auto.
-  assert (u0 = _to).
-  subst u0 u. auto.
-  assert (u1 = _value).
-  subst u1 u0 u. auto.
-  assert (u2 = _success ).
-  subst u2 u1 u0 u. auto.
-  assert (u3 = _allowance).
-  subst u3 u2 u1 u0 u. auto.
+  assert (u1 = _from) by auto.
+  assert (u2 = _to).
+  subst u2 u1. auto.
+  assert (u3 = _value).
+  subst u3 u2 u1. auto.
+  assert (u4 = _success ).
+  subst u4 u3 u2 u1. auto.
+  assert (u5 = _allowance).
+  subst u5 u4 u3 u2 u1. auto.
 
-  (* subst _from _to _value _allowance _success. *)
-  rewrite H1, H2, H3, H4, H5.
-  f_equal. auto. 
+  rewrite H1, H2, H3, H4, H5. 
+  f_equal. auto.  
 Qed.  
-
-(* Definition transferFrom_ls_template_computed: 
-                       forall (_from :  address)
-                              (_to :  address) 
-                              (_value :  uint256)
-                              (l: LedgerLRecord rec), 
-    {t: LedgerLRecord rec | t = transferFrom_ls_template_exec _from _to _value {$$ l with Ledger_LocalState := default $$}}. 
-Proof.
-    intros.
-    remember (transferFrom_ls_template_exec _from _to _value {$$ l with Ledger_LocalState := default $$}).
-
-    destruct l. repeat destruct p.
-    destruct v. repeat destruct p.
-    destruct c. repeat destruct p. idtac.
-
-    time "transferFrom_ls_template_exec unfold" unfold transferFrom_ls_template_exec in Heql0. idtac.
-    
-    time "remember" match goal with
-    | Heql0 : l0 = ?L |- _ => match L with
-                              | context [exec_state (Uinterpreter (transferFrom_ls_payload rec def ?a1 ?a2 ?a3 ?a4 ?a5 )) ?LL] => 
-                                        remember LL
-                              end
-    end. idtac.
-
-    time "transferFrom_ls_pre_payload_computed compute" vm_compute in Heql3. idtac.
-
-    time "remember" match goal with
-    | Heql0 : l0 = ?L |- _ => match L with
-                              | context [exec_state (Uinterpreter (transferFrom_ls_payload rec def ?a1 ?a2 ?a3 ?a4 ?a5 )) ?LL] => 
-                                        remember a1
-                              end
-    end. idtac.
-
-    time "remember" match goal with
-    | Heql0 : l0 = ?L |- _ => match L with
-                              | context [exec_state (Uinterpreter (transferFrom_ls_payload rec def ?a1 ?a2 ?a3 ?a4 ?a5 )) ?LL] => 
-                                        remember a2
-                              end
-    end. idtac.
-
-    time "remember" match goal with
-    | Heql0 : l0 = ?L |- _ => match L with
-                              | context [exec_state (Uinterpreter (transferFrom_ls_payload rec def ?a1 ?a2 ?a3 ?a4 ?a5 )) ?LL] => 
-                                        remember a3
-                              end
-    end. idtac.
-
-    time "remember" match goal with
-    | Heql0 : l0 = ?L |- _ => match L with
-                              | context [exec_state (Uinterpreter (transferFrom_ls_payload rec def ?a1 ?a2 ?a3 ?a4 ?a5 )) ?LL] => 
-                                        remember a4
-                              end
-    end. idtac.
-
-    time "remember" match goal with
-    | Heql0 : l0 = ?L |- _ => match L with
-                              | context [exec_state (Uinterpreter (transferFrom_ls_payload rec def ?a1 ?a2 ?a3 ?a4 ?a5 )) ?LL] => 
-                                        remember a5
-                              end
-    end. idtac.
-
-    assert (forall l, exec_state (sRReader (ULtoRValue u2)) l = l). 
-    intros. 
-    subst u2. auto.
-
-    rewrite H in Heql0.
-
-    assert (l0 = exec_state (UinterpreterUnf listInfinite (transferFrom_ls_payload rec def u u0 u1 u2 u3)) l3).
-    rewrite Heql0.
-    match goal with
-    | |- context[if ?b then _ else _] => destruct b; auto
-    end. (* clear Heql0 H. *)
-
-
-    assert (u = local_left_field _ _ _ ("_from", 1%nat)) by auto.
-    assert (u0 = local_left_field _ _ _ ("_to", 1%nat)).
-    subst u0 u. auto.
-    assert (u1 = local_left_field _ _ _ ("_value", 1%nat)).
-    subst u1 u0 u. auto.
-    assert (u2 = local_left_field _ _ _ ("success", 1%nat)).
-    subst u2 u1 u0 u. auto.
-    assert (u3 = local_left_field _ _ _ ("allowance", 1%nat)).
-    subst u3 u2 u1 u0 u. auto.
-
-    rewrite H1, H2, H3, H4, H5 in H0.
-    rewrite Heql3 in H0.
-    (* clear H1 H3 H H2 H4.     *)
-
-    clear Heql0.
-    match goal with
-    | H: l0 = ?LL |- _ => refine (exist _ LL _)
-    end. auto.
-
-Defined. *)
 
 (* payload *)
 
@@ -268,16 +177,18 @@ Definition transferFrom_ls_payload_exec (_from : ULValue address)
   let_term_of_2_fast @transferFrom_ls_payload_exec_sig (transferFrom_ls_payload_exec_sig  _from _to _value _success _allowance l).
 Defined.
 
-Definition transferFrom_ls_payload_prf (_from : ULValue address) 
+Lemma transferFrom_ls_payload_prf : forall (_from : ULValue address) 
                                        (_to : ULValue address) 
                                        (_value : ULValue uint256)
                                        (_success: ULValue boolean) 
                                        (_allowance : ULValue uint256)
-                                       (l : LedgerLRecord rec) :
+                                       (l : LedgerLRecord rec) ,
       transferFrom_ls_payload_exec _from _to _value  _success _allowance l = 
       exec_state (Uinterpreter (@transferFrom_ls_payload rec def _  _from _to _value _success _allowance)) l.
+Proof. 
+  intros.     
   proof_of_2 transferFrom_ls_payload_exec transferFrom_ls_payload_exec_sig (transferFrom_ls_payload_exec_sig _from _to _value _success _allowance l).
-Defined.
+Qed.
 
 Tactic Notation "lift_all" "in" hyp(H) := (repeat  
 (rewrite exec_if_lift in H || 
@@ -288,46 +199,95 @@ Opaque Common.hmapFindWithDefault
        CommonInstances.addAdjustListPair
        N.add N.sub N.leb N.ltb N.eqb Z.eqb N.pow.
 
-Definition transferFrom_ls_payload_exec_computed: forall (_from_value _to_value: address)
-                                                         (_value_value : uint256)
-                                                         (l: LedgerLRecord rec),
+Definition transferFrom_ls_payload_exec_computed' (_from_value _to_value: address)
+                                                  (_value_value : uint256)
+                                                  (l: LedgerLRecord rec): True.  
+  assert (LedgerLRecord rec).
+  remember (local_left_field _ _ _ ("_from", 1%nat): ULValue address) as _from.
+  remember (local_left_field _ _ _ ("_to", 1%nat): ULValue address) as _to.
+  remember (local_left_field _ _ _ ("_value", 1%nat): ULValue uint256) as _value.
+  remember (local_left_field _ _ _ ("success", 1%nat): ULValue boolean) as _success.
+  remember (local_left_field _ _ _ ("allowance", 1%nat): ULValue uint256) as _allowance.
+  remember (transferFrom_ls_pre_payload_computed _from_value _to_value _value_value l) as pre_exec.
+  remember (transferFrom_ls_payload_exec  _from _to _value  _success _allowance pre_exec) as exec.
+
+  destruct_ledger l.
+
+  time "transferFrom_ls_payload_exec unfold" unfold transferFrom_ls_payload_exec in Heqexec. 
+  time "transferFrom_ls_pre_payload_computed unfold" unfold transferFrom_ls_pre_payload_computed in Heqpre_exec.
+
+  unfold xBoolIfElse in Heqexec.
+  unfold boolFunRec in Heqexec. idtac.  
+  subst pre_exec _from _to _value _success _allowance. idtac.
+
+  time "lift" lift_all in Heqexec. idtac.
+  time "compute" compute in Heqexec. idtac.
+  time "buint" buint_all in Heqexec. idtac.
+   
+  (* symmetry in Heql1. idtac. *)     
+  match goal with
+  | Heql1: exec = ?LL |- _ => 
+    transparent_abstract exact_no_check LL using transferFrom_ls_payload_exec_computed_curried
+  end.
+  exact I.
+Defined.
+
+
+Definition transferFrom_ls_payload_exec_computed
+                              (_from :  address)
+                              (_to :  address) 
+                              (_value :  uint256)
+                              (l: LedgerLRecord rec): LedgerLRecord rec.
+remember l as ledger. destruct_ledger l.
+refine (uncurry (f:=_GlobalClass) (transferFrom_ls_payload_exec_computed_curried _from _to _value)
+      (s, (s0, (s1, (s2, (s3, (s4,
+             (c0,
+              (m,
+               (m0,
+                (v0,
+                 (v1,
+                  (v2,
+                   (v3,
+                    (v4,
+                     (v5,
+                      (v6,
+                       (v7, (v8, (v9, (v10, (v11, (v12, (v13, (v14, (v15, (v16, (v17,
+                       l1)))))))))))))))))))))))))))%xprod).
+Defined.
+
+Lemma transferFrom_ls_payload_exec_computed_correct: forall (_from_value _to_value: address)
+                                                            (_value_value : uint256)
+                                                            (l: LedgerLRecord rec),
   let _from := local_left_field _ _ _ ("_from", 1%nat) in
   let _to := local_left_field _ _ _ ("_to", 1%nat) in
   let _value := local_left_field _ _ _ ("_value", 1%nat) in
   let _success := local_left_field _ _ _ ("success", 1%nat) in
   let _allowance := local_left_field _ _ _ ("allowance", 1%nat) in  
-  let l0 := transferFrom_ls_pre_payload_computed _from_value _to_value _value_value l in
-            {t: LedgerLRecord rec | t = transferFrom_ls_payload_exec _from _to _value  _success _allowance l0}.
-Proof.        
-    intros. 
-    remember (transferFrom_ls_payload_exec  _from _to _value  _success _allowance l0).
+  let pre_exec := transferFrom_ls_pre_payload_computed _from_value _to_value _value_value l in
+      transferFrom_ls_payload_exec_computed _from_value _to_value _value_value l = 
+      transferFrom_ls_payload_exec _from _to _value _success _allowance pre_exec.
+Proof.
+  intros.
+  
+  remember (transferFrom_ls_payload_exec  _from _to _value  _success _allowance pre_exec) as exec.
+  destruct_ledger l.  
 
-    destruct l. repeat destruct p.
-    destruct v. repeat destruct p.
-    destruct c. repeat destruct p. idtac.
+  time "transferFrom_ls_payload_exec unfold" unfold transferFrom_ls_payload_exec in Heqexec.
+  time "transferFrom_ls_pre_payload_computed unfold" unfold transferFrom_ls_pre_payload_computed in pre_exec.
 
-    time "transferFrom_ls_payload_exec unfold" unfold transferFrom_ls_payload_exec in Heql1.
-    time "transferFrom_ls_pre_payload_computed unfold" unfold transferFrom_ls_pre_payload_computed in Heql1.
+  unfold xBoolIfElse in Heqexec.
+  unfold boolFunRec in Heqexec. idtac.
 
-    unfold xBoolIfElse in Heql1.
-    unfold boolFunRec in Heql1. idtac.
+  unfold transferFrom_ls_pre_payload_computed in pre_exec.  
+  subst pre_exec _from _to _value _success _allowance. idtac.
 
-    unfold transferFrom_ls_pre_payload_computed in l0.
-    subst l0. idtac. 
-    
-    subst _from _to _value _success _allowance. idtac.
-
-    time "lift" lift_all in Heql1. idtac.
-    time "compute" compute in Heql1. idtac.
-    time "buint" buint_all in Heql1. idtac.
-    symmetry in Heql1. idtac.
+  time "lift" lift_all in Heqexec. idtac.
+  time "compute" compute in Heqexec. idtac.
+  time "buint" buint_all in Heqexec. idtac.
+  
+  auto.
+Qed. 
      
-    match goal with
-    | Heql1: ?l = l1 |- _ => exact (@exist _ _ l Heql1)
-    end.
-Defined.
-
-
 
 (* Definition transferFrom_exec_sig (_from :  address)
                                  (_to :  address) 
@@ -357,514 +317,19 @@ Definition transferFrom_prf (_from :  address)
   proof_of_2 transferFrom_exec transferFrom_exec_sig (transferFrom_exec_sig _from _to _value l).
 Defined. *)
 
-
-Lemma remove_first_expression: forall X bb b`{XDefault X} (u1: UExpression X bb) (u2 u3: UExpression X b) (l: LedgerLRecord rec),
-(forall l, exec_state (Uinterpreter (ledgerClass := LedgerLLedgerClass rec def) // {u2} //) l = exec_state (Uinterpreter // {u3} //) l) -> 
-exec_state (Uinterpreter  (ledgerClass := LedgerLLedgerClass rec def) // {u1} ; {u2} //) l = exec_state (Uinterpreter // {u1} ; {u3} //) l.
+Lemma transferFrom_exec_computed: forall
+                            (_from :  address)
+                            (_to :  address)
+                            (_value : uint256)
+                            (l: LedgerLRecord rec), 
+      exec_state (Uinterpreter (@transferFrom rec def _ _ _ _  _from _to _value))  {$$ l with Ledger_LocalState := default $$} =
+      transferFrom_ls_payload_exec_computed _from _to _value l. 
 Proof.
   intros.
-  erewrite <- E_strict_bind_exec_P_helper; [|reflexivity|reflexivity|reflexivity].
-  (* erewrite <- E_err_arbitrary_false_P_helper. *)
-
-  erewrite <- E_strict_bind_exec_P_helper; [|reflexivity|reflexivity|reflexivity].
-  (* erewrite <- E_err_arbitrary_false_P_helper. *)
-  match goal with
-  | |- context [if ?b then _ else _] => destruct b
-  end.
-  - reflexivity.
-  - eapply H0.
-Qed.
-
-Lemma remove_second_expression: forall X bb b`{XDefault X} (u1: UExpression X bb) (u2 u3: UExpression X b) (l: LedgerLRecord rec),
-(forall l, exec_state (Uinterpreter (ledgerClass := LedgerLLedgerClass rec def) // {u2} //) l = 
-           exec_state (Uinterpreter // {u3} //) l) -> 
-(forall l, isError (eval_state (Uinterpreter (ledgerClass := LedgerLLedgerClass rec def) // {u2} //) l) = 
-           isError (eval_state (Uinterpreter // {u3} //) l)) ->
-exec_state (Uinterpreter  (ledgerClass := LedgerLLedgerClass rec def) // {u2} ; {u1} //) l = 
-exec_state (Uinterpreter // {u3} ; {u1} //) l.
-Proof.
-  intros.
-  erewrite <- E_strict_bind_exec_P_helper; [|reflexivity|reflexivity|reflexivity].
-  (* erewrite <- E_err_arbitrary_false_P_helper. *)
-
-  erewrite <- E_strict_bind_exec_P_helper; [|reflexivity|reflexivity|reflexivity].
-  (* erewrite <- E_err_arbitrary_false_P_helper. *)
-  rewrite H1.
-  match goal with
-  | |- context [if ?b then _ else _] => remember b
-  end.
-  setoid_rewrite <- Heqb0. destruct b0.
-  - eapply H0.
-  - rewrite H0. reflexivity.
-Qed.
-
-Lemma remove_first_assigment: forall A X b`{XDefault X}`{LocalStateField mapping rec A}`{XDefault A}  
- (s:string) (f1 f2: ULValue A -> UExpression X b) (l: LedgerLRecord rec),
-(forall ll lv (H: lv = eval_state (new_lvalue s) l), exec_state (Uinterpreter (f1 lv)) ll = exec_state (Uinterpreter (f2 lv)) ll) -> 
-exec_state (Uinterpreter (dynamicAssignL s f1)) l = exec_state (Uinterpreter (dynamicAssignL s f2)) l.
-Proof.
-  intros.
-  unfold dynamicAssignL.
-  erewrite <- E_dynamic_binding_exec_P_helper; [|reflexivity|reflexivity|reflexivity].  
-  erewrite <- E_dynamic_binding_exec_P_helper; [|reflexivity|reflexivity|reflexivity].    
-  eapply H2. reflexivity.
-Qed.
-
-Lemma var_assigment_ass: forall A X b bb`{XDefault X}`{LocalStateField mapping rec A}`{XDefault A}  
- (s:string) (u: UExpression X b) (x: URValue A bb) (l: LedgerLRecord rec),
-exec_state (Uinterpreter (ledgerClass := LedgerLLedgerClass rec def) (dynamicAssignL s (fun lv => // {lv} := {x} ; {u} //))) l =  
-exec_state (Uinterpreter // {dynamicAssignL s (fun lv => // {lv} := {x} // ) } ; {u} // ) l.
-Proof.
-  intros.
-  unfold dynamicAssignL.
-  erewrite <- E_dynamic_binding_exec_P_helper; [|reflexivity|reflexivity|reflexivity].
-  symmetry.
-  erewrite <- E_strict_bind_exec_P_helper; [|reflexivity|reflexivity|reflexivity].
-  erewrite <- E_dynamic_binding_exec_P_helper; [|reflexivity|reflexivity|reflexivity].
-  erewrite <- E_strict_bind_exec_P_helper; [|reflexivity|reflexivity|reflexivity].
-  erewrite <- E_dynamic_binding_eval_P_helper; [|reflexivity|reflexivity|reflexivity].
-
+  rewrite transferFrom_ls_template_exec_correct.
+  rewrite transferFrom_ls_payload_exec_computed_correct.
+  rewrite transferFrom_ls_payload_prf.
+  rewrite <- transferFrom_ls_template_by_payload.
+  rewrite transferFrom_ls_template_exec_prf.
   reflexivity.
 Qed.
-
-
-Lemma double_assigment_exec': forall A`{LocalStateField mapping rec A}`{XDefault A}  
-  (lv: ULValue A) (a a0: A) (l: LedgerLRecord rec),
-exec_state (rpureLWriterN lv a0) (exec_state (rpureLWriterN lv a) l) =
-exec_state (rpureLWriterN lv a0) l.
-Admitted.
-
-Lemma double_assigment_exec: forall A X b`{XDefault X}`{LocalStateField mapping rec A}`{XDefault A}  
- (u: UExpression X b) (lv: ULValue A) (x: URValue A false) (y: URValue A false) (l: LedgerLRecord rec),
-exec_state (sRReader x) l = l -> 
-(forall l, exec_state (sRReader y) l = l) -> 
-(forall a, eval_state (sRReader y) (exec_state (rpureLWriterN lv a) l) = eval_state (sRReader y) l) ->
-exec_state (Uinterpreter (ledgerClass := LedgerLLedgerClass rec def) 
-                         // {lv} := {x} ; {lv} := {y} ; {u} // ) l =
-exec_state (Uinterpreter (ledgerClass := LedgerLLedgerClass rec def) 
-                         // {lv} := {y} ; {u} // ) l.
-Proof.
-  intros.
-  erewrite <- E_strict_bind_exec_P_helper; [|reflexivity|reflexivity|reflexivity].
-  erewrite <- E_err_arbitrary_false_P_helper.
-  erewrite <- E_assign_exec_false_P_helper with (r:=x); [|reflexivity|reflexivity|reflexivity].
-  rewrite H2.
-  remember (toValue (eval_state (sRReader x) l)).
-  erewrite <- E_strict_bind_exec_P_helper; [|reflexivity|reflexivity|reflexivity].
-  erewrite <- E_strict_bind_exec_P_helper; [|reflexivity|reflexivity|reflexivity].
-  erewrite <- ?E_err_arbitrary_false_P_helper.
-  erewrite <- E_assign_exec_false_P_helper with (r:=y); [|reflexivity|reflexivity|reflexivity].
-  erewrite <- E_assign_exec_false_P_helper with (r:=y); [|reflexivity|reflexivity|reflexivity].
-  remember (toValue (eval_state (sRReader y) l)).
-  rewrite ?H3.
-
-  f_equal.
-  rewrite H4. rewrite <- Heqa0.
-  erewrite double_assigment_exec' with (A:=A); auto.
-Qed.
-
-Lemma double_assigment_eval: forall A X b`{XDefault X}`{LocalStateField mapping rec A}`{XDefault A}  
- (u: UExpression X b) (lv: ULValue A) (x: URValue A false) (y: URValue A false) (l: LedgerLRecord rec),
-exec_state (sRReader x) l = l -> 
-(forall l, exec_state (sRReader y) l = l) -> 
-(forall a, eval_state (sRReader y) (exec_state (rpureLWriterN lv a) l) = eval_state (sRReader y) l) ->
-eval_state (Uinterpreter (ledgerClass := LedgerLLedgerClass rec def) 
-                         // {lv} := {x} ; {lv} := {y} ; {u} // ) l =
-eval_state (Uinterpreter (ledgerClass := LedgerLLedgerClass rec def) 
-                         // {lv} := {y} ; {u} // ) l.
-Proof.                         
-  intros.
-  erewrite <- E_strict_bind_eval_P_helper; [|reflexivity|reflexivity|reflexivity].
-  erewrite <- E_assign_eval_P_helper; [|reflexivity].
-  remember (eval_state (sRReader x) l).
-  dependent destruction c.
-
-  erewrite <- E_assign_exec_false_P_helper with (r:=x); [|reflexivity|reflexivity|reflexivity].
-  rewrite H2.
-  remember (toValue (eval_state (sRReader x) l)).
-
-  erewrite <- E_strict_bind_eval_P_helper; [|reflexivity|reflexivity|reflexivity].
-  erewrite <- E_assign_eval_P_helper; [|reflexivity].
-  symmetry.
-  erewrite <- E_strict_bind_eval_P_helper; [|reflexivity|reflexivity|reflexivity].
-  erewrite <- E_assign_eval_P_helper; [|reflexivity].
-  rewrite H4.
-  remember (eval_state (sRReader y) l).
-  dependent destruction c.
-
-  erewrite <- E_assign_exec_false_P_helper with (r:=y); [|reflexivity|reflexivity|reflexivity].
-  erewrite <- E_assign_exec_false_P_helper with (r:=y); [|reflexivity|reflexivity|reflexivity].
-  remember (toValue (eval_state (sRReader y) l)).
-  rewrite ?H3. rewrite H4. 
-  change (toValue (ControlValue false a)) with a.
-  erewrite double_assigment_exec' with (A:=A); auto.
-  replace a2 with a.
-  remember (eval_state (UinterpreterUnf listInfinite u) (exec_state (rpureLWriterN lv a) l)).
-  dependent destruction c; auto.
-
-  remember (eval_state (sRReader y) l).
-  dependent destruction c.
-  inversion Heqc0. auto.
-Qed.
-
-
-Lemma transferFrom_ls_template_exec_correct_helper: forall l l' (u: URValue _ false),
-    l.(Ledger_MainState) = l'.(Ledger_MainState) ->
-    l.(Ledger_VMState) = l'.(Ledger_VMState) ->
-    eval_state (sRReader u) l = eval_state (sRReader u) l' ->
-    (forall l, (exec_state (sRReader u) l).(Ledger_MainState) = l.(Ledger_MainState)) ->
-    eval_state (sRReader (URIndex \\ msg->sender \\ (URIndex u (allowed_right rec def)))) l = 
-    eval_state (sRReader (URIndex \\ msg->sender \\ (URIndex u (allowed_right rec def)))) l'.
-Proof.
-  intros.
-  destruct l. repeat destruct p.
-  destruct c. repeat destruct p.
-  destruct v. repeat destruct p. 
-
-  destruct l'. repeat destruct p.
-  destruct c. repeat destruct p.
-  destruct v. repeat destruct p.
-
-  compute in H. compute in H0.
-  inversion H. subst x x0 x1 x2 x3 x4. 
-  inversion H0. subst x5 x6 x7 x8 x9 a x10 x11 a0 t t0 x12 x13 t1 x14 x15 l1 x16.
-  clear H H0.
-
-  assert (forall X (c1: ControlResult X false) c2,
-          toValue c1 = toValue c2 -> c1 = c2 ).
-  -
-    intros. 
-    dependent destruction c2; dependent destruction c3.
-    compute in H. congruence.
-  -
-    apply H.
-    erewrite <- R_index_eval_false_P_helper; [|reflexivity|reflexivity|reflexivity].
-    symmetry.
-    erewrite <- R_index_eval_false_P_helper; [|reflexivity|reflexivity|reflexivity].
-    
-    unfold msg_sender. unfold wrapURValue.
-    unfold SML_NG32.wrapURValue.
-    erewrite <- ?R_state_exec_P_helper.
-
-    erewrite <- R_index_eval_false_P_helper; [|reflexivity|reflexivity|reflexivity].
-    symmetry.
-    erewrite <- R_index_eval_false_P_helper; [|reflexivity|reflexivity|reflexivity].
-    rewrite H1.
-
-    f_equal. f_equal. f_equal.
-
-    match goal with
-    | |- context [eval_state _ (exec_state _ ?l) = 
-                  eval_state _ (exec_state _ ?l1)]
-        => remember l; remember l1
-    end.
-
-    pose proof (H2 x).
-    pose proof (H2 x0).
-    remember (exec_state (sRReader u) x).
-    remember (exec_state (sRReader u) x0).
-    setoid_rewrite <- Heqx1 in H0.
-    setoid_rewrite <- Heqx2 in H3.
-    setoid_rewrite <- Heqx1.
-    setoid_rewrite <- Heqx2.
-        
-    destruct x1. repeat destruct p.
-    destruct c. repeat destruct p.
-    destruct v. repeat destruct p. 
-
-    destruct x2. repeat destruct p.
-    destruct c. repeat destruct p.
-    destruct v. repeat destruct p.
-
-    subst x0 x.
-    compute in H0, H3.
-
-    inversion H0.
-    subst x1 x3 x4 x5 x6 x7.
-
-    inversion H3.
-    subst x2 x38 x39 x40 x41 x42.
-    auto.
-Qed.
-
-
-Lemma transferFrom_ls_template_exec_correct: forall (_from :  address)
-                                                    (_to :  address) 
-                                                    (_value :  uint256) 
-                                                    (l : LedgerLRecord rec),
-      exec_state (Uinterpreter (@transferFrom rec def _ _ _ _  _from _to _value)) l = 
-      exec_state (Uinterpreter (@transferFrom_ls_template rec def _ _ _ _  _from _to _value)) l.
-Proof.
-  intros.
-  unfold transferFrom.
-  unfold transferFrom_ls_template.
-  unfold transferFrom_ls_payload.
-  unfold fromUReturnExpression.
-
-  eapply remove_first_assigment; intros.
-  eapply remove_first_expression; intros.
-  eapply remove_first_assigment; intros.
-  eapply remove_first_expression; intros.
-  eapply remove_first_assigment; intros.
-  eapply remove_first_expression; intros.
-  eapply remove_first_assigment; intros.
-  eapply remove_first_expression; intros.
-
-  unfold dynamicAssignL.
-  
-  match goal with
-  | |- context [@DynamicBinding _ _ _ _ _ _ _ _ _ _ _ _ _ _ _ _ _  ?f] => remember f
-  end.
-  symmetry.
-  match goal with
-  | |- context [@DynamicBinding _ _ _ _ _ _ _ _ _ _ _ _ _ _ _ _ _  ?f] => remember f
-  end.
-
-  match goal with
-  | |- context [ // {?u1} ; {?u2} //  ] => remember u1; remember u2
-  end.
-  symmetry.
-  match goal with
-  | |- context [ // {?u1} ; {?u2} //  ] => remember u1
-  end.
-
-  apply remove_second_expression with  (u1:=u2) (u2:=u3) (u3:=u1); intros.
-  
-  all: subst u3 u1 u u0.
-  1: erewrite <- E_dynamic_binding_exec_P_helper; [|reflexivity|reflexivity|reflexivity].
-  1: erewrite <- E_dynamic_binding_exec_P_helper; [|reflexivity|reflexivity|reflexivity].
-  2: erewrite <- E_dynamic_binding_err_P_helper; [|reflexivity|reflexivity|reflexivity].
-  2: erewrite <- E_dynamic_binding_err_P_helper; [|reflexivity|reflexivity|reflexivity].
-  
-  all: remember (eval_state (SML_NG32.new_lvalue "allowance") l4).  
-  all: symmetry.
-  all: match goal with
-  | |- context [ // {?x} ; {?y} := {?a} ; {?z} // ] => remember a; remember z
-  end.
-  all: remember (exec_state (SML_NG32.new_lvalue "allowance") l4).
-  
-  1: apply double_assigment_exec with 
-           (lv := u) 
-           (u := u1) (y:=u0) (l:=l5).
-  6: f_equal; apply double_assigment_eval with 
-           (lv := u) 
-           (u := u1) (y:=u0) (l:=l5).
-
-  1,6: refine LocalStateField0.
-  1,5: refine ubint_default.
-  1,4: auto.
-  1,3:  ( intros ; subst u0 lv;
-         destruct l6 ; repeat destruct p ;
-         destruct c ; repeat destruct p ;
-         destruct v ; repeat destruct p ; auto ).
-  all:  (intros; subst u u0 lv;
-    remember ((eval_state (new_lvalue "_from") l1)) ;
-    apply transferFrom_ls_template_exec_correct_helper ).
-  1,5: (destruct l5 ; repeat destruct p ;
-        destruct c ; repeat destruct p ;
-        destruct v ; repeat destruct p ; auto ).
-  1,4: (destruct l5 ; repeat destruct p ;
-        destruct c ; repeat destruct p ;
-        destruct v ; repeat destruct p ; auto).
-  1,3:  (subst u;
-    destruct l5;  repeat destruct p;
-    destruct c; repeat destruct p;
-    destruct v; repeat destruct p). 
-  1,2:  (
-    destruct l1; repeat destruct p;
-    destruct c; repeat destruct p;
-    destruct v; repeat destruct p).         
-
-  1,2:  (
-    destruct l4; repeat destruct p;
-    destruct c; repeat destruct p;
-    destruct v; repeat destruct p; auto).
-
-    Opaque Common._hmapFindWithDefault _addAdjustListPair.
-   1,2: (compute;
-    destruct l1 ; destruct l12;
-    destruct l12 ; destruct l5 ;
-    destruct l12 ; destruct l12 ; reflexivity ).
-
-    Transparent Common._hmapFindWithDefault _addAdjustListPair.
-    1,2: (subst u;
-    destruct l5; repeat destruct p;
-    destruct c; repeat destruct p;
-    destruct v; repeat destruct p;  auto ) .
-Qed.
-
-Definition transferFrom_exec_computed: forall
-                            (_from :  address)
-                            (_to :  address)
-                            (_value : uint256)
-                            (l: LedgerLRecord rec), 
-  {t: LedgerLRecord rec | t = exec_state (Uinterpreter (@transferFrom rec def _ _ _ _  _from _to _value))  {$$ l with Ledger_LocalState := default $$}}.
-  intros.
-  remember (transferFrom_ls_payload_exec_computed _from _to _value l ).  
-  unfold transferFrom_ls_payload_exec_computed in Heqs.
-  refine (exist _ (proj1_sig s) _).
-  rewrite transferFrom_ls_template_exec_correct.
-  rewrite <- transferFrom_ls_template_exec_prf.
-  rewrite transferFrom_ls_template_by_payload.
-  rewrite <- transferFrom_ls_payload_prf.
-  apply (proj2_sig).
-Defined.  
-
-
-Print transferFrom_exec_computed.
-
-
-
-
-
-(* Definition transferFrom_exec_computed: forall
-                            (_from :  address)
-                            (_to :  address)
-                            (_value : uint256)
-                            (l: LedgerLRecord rec), 
-                            {t: LedgerLRecord rec | t = transferFrom_exec _from _to _value {$$ l with Ledger_LocalState := default $$}}.
-Proof.        
-    intros. 
-    remember (transferFrom_exec _from _to _value {$$ l with Ledger_LocalState := default $$}).
-
-    destruct l. repeat destruct p.   
-    destruct v. repeat destruct p.
-    destruct c. repeat destruct p.  idtac.
-
-    unfold transferFrom_exec in Heql0. idtac.    
-
-    unfold xBoolIfElse in Heql0.
-    unfold boolFunRec in Heql0.
-
-    time "lift1" lift_all in Heql0.         
-    time "compute1" compute in Heql0.  
-    time "buint1" buint_all in Heql0.
-    symmetry in Heql0. idtac.
-    
-    match goal with
-    | Heql0: ?l = l0 |- _ => exact (@exist _ _ l Heql0)
-    end.
-Defined. *)
-
-
-
-
-
-(*eval*)
-
-(* Definition transferFrom_eval_sig (_from :  address) (_to :  address) 
-                             (_value :  uint256) (l : LedgerLRecord rec) :
-                             {t | t = eval_state (Uinterpreter (@transferFrom rec def _ _ _ _  _from _to _value)) l}.
-  unfold transferFrom. unfold dynamicAssignL.
-  unfold fromUReturnExpression.  
-  repeat auto_build_P listInfinite.
-Defined.
-
-Definition transferFrom_eval_let (_from :  address) (_to :  address) 
-                             (_value :  uint256) (l : LedgerLRecord rec) : ControlResult bool true.
-  let_term_of_2_fast @transferFrom_eval_sig (transferFrom_eval_sig _from _to _value l).
-Defined.
-
-Definition transferFrom_eval (_from :  address) (_to :  address) 
-                         (_value :  uint256)  (l : LedgerLRecord rec) : ControlResult bool true.
-  flat_term_of_2 @transferFrom_eval_let (transferFrom_eval_let _from _to _value l).
-Defined.
-
-Definition transferFrom_eval_prf (_from :  address) (_to :  address) 
-                         (_value :  uint256) (l : LedgerLRecord rec) :
-  transferFrom_eval _from _to _value l = 
-  eval_state (Uinterpreter (@transferFrom rec def _ _ _ _ _from _to _value)) l.
-  proof_of_2 transferFrom_eval transferFrom_eval_sig (transferFrom_eval_sig _from _to _value l).
-Defined. *)
-
-
-
-(* template left *)
-
-(* Definition transferFromTemplate_exec_sig1 
-                                 (_from :  address)
-                                 (_to :  address) 
-                                 (_value :  uint256) (l : LedgerLRecord rec) :
-  {t | t = exec_state (Uinterpreter (@transferFromTemplate_left rec def _ _ _ _ false (URScalar _from) false (URScalar _to) false (URScalar _value) bool )) l}.
-  unfold transferFromTemplate_left.
-  unfold wrapULExpressionL.
-  unfold wrapULExpression.
-  unfold ursus_call_with_argsL.
-
-  match goal with
-  | |- context [@ursus_call_with_args ?a1 ?a2 ?a3 ?a4 ?a5 ?a6 ?a7 ?a8 ?a9 ?a10 ?a11 ?a12 ?a13 ?a14 ?a15 ?a16 ?a17 ?a18 ?a19 ?a20] =>
-            remember (@ursus_call_with_args a1 a2 a3 a4 a5 a6 a7 a8 a9 a10 a11 a12 a13 a14 a15 a16 a17 a18 a19 a20)
-  end.
-  unfold SML_NG32.UExpressionP0_LedgerableWithArgs_obligation_1 in u.
-  change (transferFromTemplate rec def) with (fun (_from _to : address) (_value : uint256) => transferFromTemplate rec def _from _to _value) in Hequ.
-  Opaque transferFromTemplate.
-  
-  simpl in Hequ.
-  unfold SML_NG32.UExpressionP0_LedgerableWithArgs_obligation_4 in Hequ.  
-  unfold SML_NG32.UExpressionP0_LedgerableWithArgs_obligation_4 in Hequ.
-  unfold SML_NG32.UExpressionP0_LedgerableWithArgs_obligation_5 in Hequ.
-  unfold ursus_call_with_rargs0 in Hequ.
-  simpl in Hequ.
-  unfold simple_state_bind,  simple_state_unit in Hequ.
-  unfold simple_state_run in Hequ.
-  unfold compose in Hequ.
-  unfold SML_NG32.UExpressionP0_LedgerableWithArgs_obligation_7 in Hequ.
-  unfold sRReader in Hequ.
-  simpl in Hequ.
-
-  change Datatypes.list with XList.
-
-  auto_build_P listInfinite.
-  all: subst u.  
-  1: refine (exist _ (exec_state (UinterpreterUnf listInfinite (transferFromTemplate rec def _from _to _value)) l) _).
-  2: refine (exist _ (eval_state (UinterpreterUnf listInfinite (transferFromTemplate rec def _from _to _value)) l) _).
-
-  all: remember (UinterpreterUnf listInfinite (transferFromTemplate rec def _from _to _value)) as ll.
-  all: destruct ll.
-  1: unfold exec_state.
-  2: unfold eval_state.
-  all: simpl.
-  all: remember (x l) as xx.
-  all: destruct xx. 
-  all: simpl. 
-  1: reflexivity.
-  dependent destruction c; reflexivity.
-Defined.
-
-
-
-Definition transferFromTemplate_exec_sig2 
-                                 (_from :  address)
-                                 (_to :  address) 
-                                 (_value :  uint256) (l : LedgerLRecord rec) :
-  {t | t = exec_state (Uinterpreter (@transferFromTemplate_left rec def _ _ _ _ false (URScalar _from) false (URScalar _to) false (URScalar _value) bool )) l}.
-remember (proj1_sig (transferFromTemplate_exec_sig1 _from _to _value l)).
-pose proof (proj2_sig (transferFromTemplate_exec_sig1 _from _to _value l)).
-unfold transferFromTemplate_exec_sig1 in Heql0, H.
-setoid_rewrite <- Heql0 in H.
-simpl in Heql0.
-
-symmetry in Heql0.
-
-match goal with 
-| Heql0: ?L = l0 |- _ => refine (exist _ L _)
-end.
-rewrite Heql0.
-assumption.
-Defined.
-
-
-Definition transferFromTemplate_exec_sig3
-                                 (_from :  address)
-                                 (_to :  address) 
-                                 (_value :  uint256) (l : LedgerLRecord rec) :
-  {t | t = exec_state (Uinterpreter (@transferFromTemplate_left rec def _ _ _ _ false (URScalar _from) false (URScalar _to) false (URScalar _value) bool )) l}.
-remember (proj1_sig (transferFromTemplate_exec_sig2 _from _to _value l)).
-pose proof (proj2_sig (transferFromTemplate_exec_sig2 _from _to _value l)).
-unfold transferFromTemplate_exec_sig2 in Heql0, H.
-setoid_rewrite <- Heql0 in H.
-simpl in Heql0.
-Admitted.
-
-
-Transparent transferFromTemplate. *)
